Add crash to corr2 definition

src/PermHoare.v
@@ -1,5 +1,5 @@
 Require Import Mem Pred.
-Require Import PermProg PermSec.
+Require Export PermProgMonad PermPredCrash.
 Require Import List.
 Require Import Morphisms.
 Require Import Word.
@@ -13,12 +13,13 @@ Definition pair_args_helper (A B C:Type) (f: A->B->C) (x: A*B) := f (fst x) (snd
 
 Definition donecond (T: Type) := tagged_disk -> block_mem -> T -> Prop.
 
-Definition corr2 (T: Type) pr (pre: donecond T -> block_mem -> @pred _ _ tagged_block) (p: prog T) :=
-  forall d bm tr tr' donec out,
-    pre donec bm d
+Definition corr2 (T: Type) pr (pre: donecond T -> @pred _ PeanoNat.Nat.eq_dec valuset -> block_mem ->  @pred _ _ valuset) (p: prog T) :=
+  forall d bm tr tr' donec crashc out,
+    pre donec crashc bm d
   -> exec pr tr d bm p out tr'
-  -> (exists d' bm' v, out = Finished d' bm' v /\
-                 donec d' bm' v) /\
+  -> ((exists d' bm' v, out = Finished d' bm' v /\
+                  donec d' bm' v) \/
+    (exists d', out = Crashed d' /\ crashc d'))/\
     permission_secure d bm pr p.
 
 Notation "{{ pr : pre }} p" := (corr2 pr pre p)
@@ -54,10 +55,29 @@ Notation "{< e1 .. e2 , 'PERM' : pr 'PRE' : pre 'POST' : post >} p1" :=
            post bm' F_ r_ *
            [[ done'_ = done_ ]])%pred (rx r_) ]]
      )) .. ))
-   )%pred) (* Weird scoping problem *)
+   )%pred)
    (Bind p1 rx)%pred)
   (at level 0, p1 at level 60, right associativity, 
    e1 closed binder, e2 closed binder).
+
+
+Notation "{< e1 .. e2 , 'PERM' : pr 'PRE' : bm pre 'POST' : bm' post 'CRASH' : crash >} p1" :=
+  (forall T (rx: _ -> prog T), corr2 pr%pred
+   (fun done_ crash_ bm =>
+    (exis (fun e1 => .. (exis (fun e2 =>
+     exists F_,
+     F_ * pre *
+     [[ sync_invariant F_ ]] *
+     [[ forall r_ , corr2 pr
+        (fun done'_ crash'_ bm' =>
+           post F_ r_ * [[ done'_ = done_ ]] * [[ crash'_ = crash_ ]])
+        (rx r_) ]] *
+     [[ (F_ * crash) =p=> crash_ ]]
+     )) .. ))
+   )%pred
+   (Bind p1 rx)%pred)
+  (at level 0, p1 at level 60, bm at level 0, bm' at level 0,
+    e1 closed binder, e2 closed binder).
 
 Notation "{< 'X' , 'PERM' : pr 'PRE' : pre 'POST' : post >} p1" :=
   (forall T (rx: _ -> prog T), corr2 pr%pred
@@ -72,11 +92,25 @@ Notation "{< 'X' , 'PERM' : pr 'PRE' : pre 'POST' : post >} p1" :=
    (Bind p1 rx)%pred)
   (at level 0, p1 at level 60, right associativity).
 
+Notation "{< 'X' , 'PERM' : pr 'PRE' : bm pre 'POST' : bm' post 'CRASH' : crash >} p1" :=
+  (forall T (rx: _ -> prog T), corr2 pr%pred
+   (fun done_ crash_ bm =>
+     exists F_,
+     F_ * pre *
+     [[ sync_invariant F_ ]] *
+     [[ forall r_ , corr2 pr
+        (fun done'_ crash'_ bm' =>
+           post F_ r_ * [[ done'_ = done_ ]] * [[ crash'_ = crash_ ]])
+        (rx r_) ]] *
+     [[ (F_ * crash) =p=> crash_ ]]
+   )%pred
+   (Bind p1 rx)%pred)
+  (at level 0, p1 at level 60, bm at level 0, bm' at level 0).
 
 Theorem pimpl_ok2:
-  forall T pr  (pre pre': donecond T -> block_mem -> @pred _ _ tagged_block) (p: prog T),
+  forall T pr  (pre pre':donecond T -> @pred _ PeanoNat.Nat.eq_dec valuset -> block_mem ->  @pred _ _ valuset) (p: prog T),
   corr2 pr pre' p ->
-  (forall done bm, pre done bm =p=>  pre' done bm) ->
+  (forall done crash bm, pre done crash bm =p=>  pre' done crash bm) ->
   corr2 pr pre p.
 Proof.
   unfold corr2; intros.
@@ -85,10 +119,10 @@ Proof.
 Qed.
 
 Theorem pimpl_ok2_cont :
-  forall T pr (pre pre': donecond T -> block_mem -> @pred _ _ tagged_block) A (k : A -> prog T) x y,
+  forall T pr (pre pre': donecond T -> @pred _ PeanoNat.Nat.eq_dec valuset -> block_mem ->  @pred _ _ valuset) A (k : A -> prog T) x y,
     corr2 pr pre' (k y) ->
-    (forall done bm, pre done bm  =p=>  pre' done bm) ->
-    (forall done bm, pre done bm  =p=> [x = y]) ->
+    (forall done crash bm, pre done crash bm  =p=>  pre' done crash bm) ->
+    (forall done crash bm, pre done crash bm  =p=> [x = y]) ->
     corr2 pr pre (k x).
 Proof.
   unfold corr2; intros.
@@ -98,9 +132,9 @@ Proof.
 Qed.
 
 Theorem pimpl_pre2:
-  forall T pr pre' (pre: donecond T -> block_mem -> @pred _ _ tagged_block) (p: prog T),
-    (forall done bm, pre done bm  =p=>  [corr2 pr (pre' done bm) p]) ->
-    (forall done bm, pre done bm  =p=> pre' done bm done bm) ->
+  forall T pr pre' (pre: donecond T -> @pred _ PeanoNat.Nat.eq_dec valuset -> block_mem ->  @pred _ _ valuset) (p: prog T),
+    (forall done crash bm, pre done crash bm  =p=>  [corr2 pr (pre' done crash bm) p]) ->
+    (forall done crash bm, pre done crash bm  =p=> pre' done crash bm done crash bm) ->
     corr2 pr pre p.
 Proof.
   unfold corr2; intros.
@@ -109,8 +143,8 @@ Proof.
 Qed.
 
 Theorem pre_false2:
-  forall T pr (pre: donecond T -> block_mem -> @pred _ _ tagged_block) (p: prog T),
-    (forall done bm, pre done bm  =p=>  [False]) ->
+  forall T pr (pre: donecond T -> @pred _ PeanoNat.Nat.eq_dec valuset -> block_mem ->  @pred _ _ valuset) (p: prog T),
+    (forall done crash bm, pre done crash bm  =p=>  [False]) ->
     corr2 pr pre p.
 Proof.
   unfold corr2; intros; exfalso.
@@ -119,8 +153,8 @@ Qed.
 
 Theorem corr2_exists:
   forall T R pr pre (p: prog R),
-    (forall (a:T), corr2 pr (fun done bm => pre done bm a) p) ->
-    corr2 pr (fun done bm => exists a:T, pre done bm a)%pred p.
+    (forall (a:T), corr2 pr (fun done crash bm => pre done crash bm a) p) ->
+    corr2 pr (fun done crash bm => exists a:T, pre done crash bm a)%pred p.
 Proof.
   unfold corr2; intros.
   destruct H0.
@@ -129,10 +163,37 @@ Qed.
 
 Theorem corr2_forall:
     forall T R pr pre (p: prog R),
-      corr2 pr (fun done bm => exists a:T, pre done bm a)%pred p ->
-  (forall (a:T), corr2 pr (fun done bm => pre done bm a) p).
+      corr2 pr (fun done crash bm => exists a:T, pre done crash bm a)%pred p ->
+  (forall (a:T), corr2 pr (fun done crash bm => pre done crash bm a) p).
 Proof.
   unfold corr2; intros.
   eapply H; eauto.
   exists a; auto.
 Qed.
+
+  Theorem corr2_equivalence :
+    forall T pr (p p': prog T) pre,
+      corr2 pr pre p' ->
+      prog_equiv p p' ->
+      corr2 pr pre p.
+  Proof.
+    unfold corr2; intros.
+    match goal with
+    | [ H: _ ~= _ |- _ ] =>
+      edestruct H; eauto
+    end.
+    edestruct H; eauto.
+    intuition.
+    eapply security_equivalence; eauto.
+    cleanup.
+    eapply security_equivalence; eauto.
+  Qed.
+
+Ltac monad_simpl_one :=
+  match goal with
+  | [ |- corr2 _ _ (Bind (Bind _ _) _) ] =>
+    eapply corr2_equivalence;
+    [ | apply bind_assoc ]
+  end.
+
+Ltac monad_simpl := repeat monad_simpl_one.
