src/PermAsyncDisk.v
@@ -1,0 +1,211 @@
+Require Import Arith.
+Require Import Word.
+Require Import List.
+Require Import Mem.
+Require Import Eqdep_dec.
+Require Import FunctionalExtensionality.
+
+Set Implicit Arguments.
+
+(* Disk value and address types  *)
+
+Notation "'valubytes_real'" := (4 * 1024)%nat. (* 4KB *)
+Notation "'valulen_real'" := (valubytes_real * 8)%nat.
+
+Module Type VALULEN.
+  Parameter valulen : nat.
+  Parameter valubytes : nat.
+  Axiom valulen_is : valulen = valulen_real.
+  Axiom valubytes_is : valubytes = valubytes_real.
+End VALULEN.
+
+Module Valulen : VALULEN.
+  Definition valulen := valulen_real.
+  Definition valubytes := valubytes_real.
+  Theorem valulen_is: valulen = valulen_real.
+  Proof.
+    auto.
+  Qed.
+  Theorem valubytes_is: valubytes = valubytes_real.
+  Proof.
+    auto.
+  Qed.
+End Valulen.
+
+Definition addrlen := 64.
+Notation "'valulen'" := (Valulen.valulen).
+Notation "'valulen_is'" := (Valulen.valulen_is).
+Notation "'valu'" := (word valulen).
+
+Theorem valulen_nonzero : valulen <> 0.
+Proof.
+  rewrite valulen_is.
+  compute.
+  apply Nat.neq_succ_0.
+Qed.
+
+Theorem valulen_gt_0 : valulen > 0.
+Proof.
+  generalize valulen_nonzero.
+  generalize valulen.
+  destruct n; intuition.
+Qed.
+
+Theorem valulen_wordToNat_natToWord : # (natToWord addrlen valulen) = valulen.
+Proof.
+  rewrite valulen_is.
+  compute.
+  reflexivity.
+Qed.
+
+(* tight bound for valulen *)
+Theorem valulen_bound : valulen < pow2 16.
+Proof.
+  eapply Nat.lt_le_trans with (m := pow2 15 + 1).
+  rewrite valulen_is.
+  compute; auto.
+  apply pow2_le_S.
+Qed.
+
+
+Notation "'addr'" := nat.
+Notation "'waddr'" := (word addrlen).
+
+Definition addr_eq_dec := Nat.eq_dec.
+Definition waddr_eq_dec := @weq addrlen.
+
+Definition waddrring := wring addrlen.
+Add Ring waddrring : waddrring (decidable (weqb_sound addrlen), constants [wcst]).
+
+
+Definition owner := nat.
+Definition block := valu.
+
+Inductive tag :=
+(* | Nothing : tag *)
+| Public : tag
+| Private : owner -> tag.
+
+Definition tag_dec : forall (t t': tag), {t = t'}+{t <> t'}.
+  intros; destruct t, t'; auto; try solve [right; congruence].
+  destruct (Nat.eq_dec o o0); subst; auto; right; congruence.
+Defined.
+
+Definition tagged_block := (tag * block)%type.
+Definition valuset := (tagged_block * list tagged_block)%type.
+
+(* Async-disk *)
+Definition rawdisk := @mem addr addr_eq_dec valuset.
+Definition vsmerge (vs : valuset) : list tagged_block := fst vs :: snd vs.
+
+
+(* Hashing *)
+Definition hashlen := 32.
+Parameter hash_fwd : forall sz, word sz -> word hashlen.
+Definition default_valu : valu := $0.
+Definition default_hash := hash_fwd default_valu.
+
+(* A hashmap holds all keys that Hash has been called on, maps hash values to keys. *)
+Inductive hashmap : Type :=
+  | empty_hashmap : hashmap
+  | upd_hashmap : hashmap -> word hashlen -> { sz : nat & word sz } -> hashmap.
+
+Definition upd_hashmap' hm h sz k : hashmap :=
+  upd_hashmap hm h (existT _ sz k).
+
+Fixpoint hashmap_get hm h : option {sz : nat & word sz} :=
+  if (weq h default_hash)
+    then Some (existT _ _ default_valu) else
+    (match hm with
+    | empty_hashmap => None
+    | upd_hashmap hm' h' k' =>  if (weq h' h)
+                                then Some k'
+                                else hashmap_get hm' h
+    end).
+
+
+Lemma upd_hashmap_eq : forall hm h k,
+  h <> default_hash ->
+  hashmap_get (upd_hashmap hm h k) h = Some k.
+Proof.
+  intros.
+  unfold hashmap_get.
+  destruct (weq h default_hash);
+  destruct (weq h h); intuition.
+Qed.
+
+Lemma upd_hashmap'_eq : forall hm h sz k,
+  h <> default_hash ->
+  hashmap_get (upd_hashmap' hm h k) h = Some (existT _ sz k).
+Proof.
+  intros.
+  unfold upd_hashmap'.
+  apply upd_hashmap_eq; auto.
+Qed.
+
+Hint Rewrite upd_hashmap_eq.
+
+
+Definition hash_safe hm h sz (k : word sz) :=
+  hashmap_get hm h = None \/ hashmap_get hm h = Some (existT _ _ k).
+
+(* Converting between hash and valu.*)
+Lemma hashlen_valulen: hashlen + (valulen - hashlen) = valulen.
+Proof.
+  rewrite valulen_is; auto.
+Qed.
+
+Definition hash_to_valu (h: word hashlen) : valu.
+  set (zext h (valulen-hashlen)) as r.
+  rewrite hashlen_valulen in r.
+  apply r.
+Defined.
+
+Lemma hash_to_valu_inj : forall a b,
+  hash_to_valu a = hash_to_valu b ->
+  a = b.
+  unfold hash_to_valu.
+  unfold eq_rec_r, eq_rec.
+  rewrite <- hashlen_valulen.
+  intros.
+  rewrite <- (eq_rect_eq_dec eq_nat_dec) in H.
+  rewrite <- (eq_rect_eq_dec eq_nat_dec) in H.
+  unfold zext in *.
+  apply combine_inj in H.
+  intuition.
+Qed.
+
+
+Definition sync_mem AT AEQ (m : @mem AT AEQ valuset) : @mem AT AEQ valuset :=
+  fun a => match m a with
+    | None => None
+    | Some (v, _) => Some (v, nil)
+    end.
+
+Definition sync_addr AT AEQ (m : @mem AT AEQ valuset) a : @mem AT AEQ valuset :=
+  fun a' => if AEQ a a' then
+    match m a with
+    | None => None
+    | Some (v, _) => Some (v, nil)
+    end else m a'.
+
+Lemma sync_addr_ne : forall AT AEQ (m : @mem AT AEQ valuset) a a',
+  a <> a' ->
+  (sync_addr m a) a' = m a'.
+Proof.
+  unfold sync_addr; intros.
+  destruct (AEQ a a'); try congruence.
+Qed.
+
+Lemma sync_addr_eq : forall AT AEQ (m : @mem AT AEQ valuset) a a' vs,
+  a = a' ->
+  m a' = Some vs ->
+  (sync_addr m a) a' = Some (fst vs, nil).
+Proof.
+  unfold sync_addr; intros; subst.
+  destruct (AEQ a' a'); try congruence.
+  destruct (m a'); try congruence.
+  inversion H0; subst.
+  destruct vs; auto.
+Qed.
+
